modular structs/vprop: a first try
expressive enough for a toy allocator?
improve with vdep/vrefine combinators?

lib_list/Selectors.LList.fst
@@ -6,6 +6,7 @@ module Mem = Steel.Memory
 open Steel.Effect.Atomic
 open Steel.Effect
 open Steel.Reference
+//open Impl.Core
 
 #push-options "--__no_positivity"
 noeq
@@ -15,311 +16,436 @@ type cell (a: Type0) = {
 }
 #pop-options
 
-let next #a (c:cell a) : t a = c.next
-let data #a (c:cell a) : a = c.data
+let get_next #a (c:cell a) : t a = c.next
+let get_data #a (c:cell a) : a = c.data
 let mk_cell #a (n: t a) (d:a) = {
   next = n;
   data = d
 }
 
-(* AF: Need to put that in the standard library at some point *)
-let null_llist #a = null
-let is_null #a ptr = is_null ptr
+let null_t #a = null
+let is_null_t #a ptr = is_null ptr
 
-let rec llist_sl' (#a:Type) (ptr:t a)
-                         (l:list (cell a))
-    : Tot slprop (decreases l)
-    =
-    match l with
-    | [] ->
-      Mem.pure (ptr == null_llist)
+let rec llist_sl' (#a:Type) (p: a -> vprop) (ptr: t a) (l: list (cell a))
+  : Tot slprop (decreases l)
+  =
+  match l with
+  | [] -> Mem.pure (ptr == null_t)
+  | hd :: tl ->
+    pts_to_sl ptr full_perm hd `Mem.star`
+    llist_sl' p (get_next hd) tl `Mem.star`
+    hp_of (p (get_data hd))
 
-    | hd :: tl ->
-      pts_to_sl ptr full_perm hd `Mem.star`
-      llist_sl' (next hd) tl `Mem.star`
-      Mem.pure (ptr =!= null_llist)
+let llist_sl p ptr = Mem.h_exists (llist_sl' p ptr)
 
+// BETA
+let ind_llist_sl' (#a: Type0) (r: ref (t a)) (p: t a) : slprop u#1
+  =
+  llist_sl #a (fun _ -> to_vprop (pts_to_sl r full_perm p)) p
+let ind_llist_sl (#a: Type0) (r: ref (t a))
+  = Mem.h_exists (ind_llist_sl' r)
 
-let llist_sl ptr = Mem.h_exists (llist_sl' ptr)
+let normal_llist_sl (#a: Type0) (ptr : t a) : slprop u#1
+  = llist_sl #a (fun _ -> emp) ptr
 
+let tree_llist_sl (#a: Type0) (ptr : t (Impl.Core.t a)) : slprop u#1
+  = llist_sl #(Impl.Core.t a)
+    (fun elem -> to_vprop (Impl.Core.tree_sl #a elem)) ptr
 
-let rec datas (#a:Type) (l:list (cell a)) : list a =
+let llist_llist_sl (#a: Type0) (ptr : t (t a)) : slprop u#1
+  = llist_sl #(t a)
+    (fun elem -> to_vprop (llist_sl #a (fun _ -> emp) elem)) ptr
+
+let rec llist_view (#a:Type) (l:list (cell a)) : list a =
   match l with
   | [] -> []
-  | hd::tl -> data hd :: datas tl
+  | hd::tl -> get_data hd :: llist_view tl
 
-val llist_sel_cell' (#a:Type0) (ptr:t a) : selector' (list (cell a)) (llist_sl ptr)
+val llist_sel_cell' (#a:Type0) (p: a -> vprop) (ptr:t a) : selector' (list (cell a)) (llist_sl p ptr)
 
-let llist_sel_cell' #a ptr = fun h -> id_elim_exists (llist_sl' ptr) h
+let llist_sel_cell' #a p ptr =
+  fun h -> id_elim_exists (llist_sl' p ptr) h
 
-let llist_sl'_witinv (#a:Type) (ptr:t a) : Lemma (is_witness_invariant (llist_sl' ptr))
+let llist_sl'_witinv (#a:Type) (p: a -> vprop) (ptr:t a) :
+  Lemma (is_witness_invariant (llist_sl' p ptr))
   = let rec aux (ptr:t a) (x y:list (cell a)) (m:mem) : Lemma
-        (requires interp (llist_sl' ptr x) m /\ interp (llist_sl' ptr y) m)
+        (requires
+          interp (llist_sl' p ptr x) m /\
+          interp (llist_sl' p ptr y) m)
         (ensures x == y)
         (decreases x)
-    = match x with
-      | [] -> begin match y with
-         | [] -> ()
-         | hd::tl ->
-           Mem.pure_interp (ptr == null_llist) m;
-           Mem.pure_star_interp
-             (pts_to_sl ptr full_perm hd `Mem.star` llist_sl' (next hd) tl)
-             (ptr =!= null_llist) m;
-           Mem.pure_interp (ptr =!= null_llist) m
-
-       end
-      | hd1::tl1 -> begin match y with
-        | [] ->
-           Mem.pure_interp (ptr == null_llist) m;
-           Mem.pure_star_interp
-             (pts_to_sl ptr full_perm hd1 `Mem.star` llist_sl' (next hd1) tl1)
-             (ptr =!= null_llist) m;
-           Mem.pure_interp (ptr =!= null_llist) m
-        | hd2::tl2 ->
-           pts_to_witinv ptr full_perm;
-           aux (next hd1) tl1 tl2 m
-      end
-
+    =
+    match x with
+    | [] -> begin match y with
+      | [] -> ()
+      | hd::tl ->
+        Mem.pure_interp (ptr == null_t) m;
+        //let p1 = pts_to_sl ptr full_perm hd in
+        //let p2 = llist_sl' p (get_next hd) tl in
+        //let p3 = hp_of (p (get_data hd)) in
+        //Mem.affine_star (p1 `Mem.star` p2) p3 m;
+        //Mem.affine_star p1 p2 m;
+        pts_to_not_null ptr full_perm hd m
+    end
+    | hd1::tl1 -> begin match y with
+      | [] ->
+        Mem.pure_interp (ptr == null_t) m;
+        //let p1 = pts_to_sl ptr full_perm hd1 in
+        //let p2 = llist_sl' p (get_next hd1) tl1 in
+        //let p3 = hp_of (p (get_data hd1)) in
+        //Mem.affine_star (p1 `Mem.star` p2) p3 m;
+        //Mem.affine_star p1 p2 m;
+        pts_to_not_null ptr full_perm hd1 m
+     | hd2::tl2 ->
+        pts_to_witinv ptr full_perm;
+        aux (get_next hd1) tl1 tl2 m
+    end
     in Classical.forall_intro_3 (Classical.move_requires_3 (aux ptr))
 
-let llist_sel_depends_only_on (#a:Type0) (ptr:t a)
-  (m0:Mem.hmem (llist_sl ptr)) (m1:mem{disjoint m0 m1})
-  : Lemma (llist_sel_cell' ptr m0 == llist_sel_cell' ptr (Mem.join m0 m1))
-  = let m':Mem.hmem (llist_sl ptr) = Mem.join m0 m1 in
-    let l1 = Ghost.reveal (id_elim_exists (llist_sl' ptr) m0) in
-    let l2 = Ghost.reveal (id_elim_exists (llist_sl' ptr) m') in
+let llist_sel_depends_only_on (#a:Type0) (p : a -> vprop) (ptr:t a)
+  (m0:Mem.hmem (llist_sl p ptr)) (m1:mem{disjoint m0 m1})
+  : Lemma (llist_sel_cell' p ptr m0 == llist_sel_cell' p ptr (Mem.join m0 m1))
+  = let m':Mem.hmem (llist_sl p ptr) = Mem.join m0 m1 in
+    let l1 = Ghost.reveal (id_elim_exists (llist_sl' p ptr) m0) in
+    let l2 = Ghost.reveal (id_elim_exists (llist_sl' p ptr) m') in
 
-    llist_sl'_witinv ptr;
-    Mem.elim_wi (llist_sl' ptr) l1 l2 m'
+    llist_sl'_witinv p ptr;
+    Mem.elim_wi (llist_sl' p ptr) l1 l2 m'
 
-let llist_sel_depends_only_on_core (#a:Type0) (ptr:t a)
-  (m0:Mem.hmem (llist_sl ptr))
-  : Lemma (llist_sel_cell' ptr m0 == llist_sel_cell' ptr (core_mem m0))
-  = let l1 = Ghost.reveal (id_elim_exists (llist_sl' ptr) m0) in
-    let l2 = Ghost.reveal (id_elim_exists (llist_sl' ptr) (core_mem m0)) in
-    llist_sl'_witinv ptr;
-    Mem.elim_wi (llist_sl' ptr) l1 l2 (core_mem m0)
+let llist_sel_depends_only_on_core (#a:Type0) (p : a -> vprop) (ptr:t a)
+  (m0:Mem.hmem (llist_sl p ptr))
+  : Lemma (llist_sel_cell' p ptr m0 == llist_sel_cell' p ptr (core_mem m0))
+  = let l1 = Ghost.reveal (id_elim_exists (llist_sl' p ptr) m0) in
+    let l2 = Ghost.reveal (id_elim_exists (llist_sl' p ptr) (core_mem m0)) in
+    llist_sl'_witinv p ptr;
+    Mem.elim_wi (llist_sl' p ptr) l1 l2 (core_mem m0)
 
-val llist_sel_cell (#a:Type0) (r:t a) : selector (list (cell a)) (llist_sl r)
+val llist_sel_cell (#a:Type0) (p : a -> vprop) (r:t a) : selector (list (cell a)) (llist_sl p r)
 
-let llist_sel_cell #a ptr =
-  Classical.forall_intro_2 (llist_sel_depends_only_on ptr);
-  Classical.forall_intro (llist_sel_depends_only_on_core ptr);
-  llist_sel_cell' ptr
+let llist_sel_cell #a p ptr =
+  Classical.forall_intro_2 (llist_sel_depends_only_on p ptr);
+  Classical.forall_intro (llist_sel_depends_only_on_core p ptr);
+  llist_sel_cell' p ptr
+
+let llist_sel #a p ptr =
+  fun h -> llist_view (llist_sel_cell p ptr h)
 
 
-let llist_sel ptr = fun h -> datas (llist_sel_cell ptr h)
 
-#push-options "--fuel 1 --ifuel 1"
+let llist_sel_interp (#a:Type0) (p : a -> vprop) (ptr:t a) (l:list (cell a)) (m:mem) : Lemma
+  (requires interp (llist_sl' p ptr l) m)
+  (ensures interp (llist_sl p ptr) m /\ llist_sel_cell' p ptr m == l)
+  = intro_h_exists l (llist_sl' p ptr) m;
+    llist_sl'_witinv p ptr
 
-let llist_sel_interp (#a:Type0) (ptr:t a) (l:list (cell a)) (m:mem) : Lemma
-  (requires interp (llist_sl' ptr l) m)
-  (ensures interp (llist_sl ptr) m /\ llist_sel_cell' ptr m == l)
-  = intro_h_exists l (llist_sl' ptr) m;
-    llist_sl'_witinv ptr
-
-let intro_nil_lemma (a:Type0) (m:mem) : Lemma
+let intro_nil_lemma (a:Type0) (p : a -> vprop) (m:mem) : Lemma
     (requires interp (hp_of emp) m)
-    (ensures interp (llist_sl (null_llist #a)) m /\ llist_sel (null_llist #a) m == [])
-    = let ptr:t a = null_llist in
-      pure_interp (ptr == null_llist) m;
+    (ensures interp (llist_sl p (null_t #a)) m /\ llist_sel p (null_t #a) m == [])
+    = let ptr:t a = null_t in
+      pure_interp (ptr == null_t) m;
       let open FStar.Tactics in
-      assert (llist_sl' ptr [] == Mem.pure (ptr == null_llist)) by (norm [delta; zeta; iota]);
-      llist_sel_interp ptr [] m
+      assert (llist_sl' p ptr [] == Mem.pure (ptr == null_t)) by (norm [delta; zeta; iota]);
+      llist_sel_interp p ptr [] m
 
-let intro_llist_nil a =
-    change_slprop_2 emp (llist (null_llist #a)) ([] <: list a) (intro_nil_lemma a)
+let intro_llist_nil a p =
+    change_slprop_2 emp (llist p (null_t #a)) ([] <: list a) (intro_nil_lemma a p)
 
-let elim_nil_lemma (#a:Type0) (ptr:t a) (m:mem) : Lemma
-    (requires interp (llist_sl ptr) m /\ ptr == null_llist)
-    (ensures interp (llist_sl ptr) m /\ llist_sel ptr m == [])
-    = let l' = id_elim_exists (llist_sl' ptr) m in
-      pure_interp (ptr == null_llist) m;
-      llist_sel_interp ptr [] m
+let elim_nil_lemma (#a:Type0) (p : a -> vprop) (ptr:t a) (m:mem) : Lemma
+    (requires interp (llist_sl p ptr) m /\ ptr == null_t)
+    (ensures interp (llist_sl p ptr) m /\ llist_sel p ptr m == [])
+    = let l' = id_elim_exists (llist_sl' p ptr) m in
+      pure_interp (ptr == null_t) m;
+      llist_sel_interp p ptr [] m
 
-let elim_llist_nil #a ptr =
-  change_slprop_rel (llist ptr) (llist ptr)
+let elim_llist_nil #a p ptr =
+  change_slprop_rel (llist p ptr) (llist p ptr)
     (fun x y -> x == y /\ y == [])
-    (fun m -> elim_nil_lemma ptr m)
+    (fun m -> elim_nil_lemma p ptr m)
 
-#set-options "--z3rlimit 20"
+//#set-options "--z3rlimit 20"
 
-let lemma_cons_not_null (#a:Type) (ptr:t a) (l:list a) (m:mem) : Lemma
-    (requires interp (llist_sl ptr) m /\ llist_sel ptr m == l /\ Cons? l)
-    (ensures ptr =!= null_llist)
-    = let l' = id_elim_exists (llist_sl' ptr) m in
-      assert (interp (llist_sl' ptr l') m);
-      llist_sel_interp ptr l' m;
-      match reveal l' with
-      | hd::tl ->
-          let p = pts_to_sl ptr full_perm (hide hd) `Mem.star` llist_sl' (next hd) tl in
-          pure_star_interp p (ptr =!= null_llist) m
+let lemma_cons_not_null (#a:Type) (p : a -> vprop) (ptr:t a) (l:list a) (m:mem) : Lemma
+  (requires interp (llist_sl p ptr) m /\ llist_sel p ptr m == l /\ Cons? l)
+  (ensures ptr =!= null_t)
+  = let l' = id_elim_exists (llist_sl' p ptr) m in
+    assert (interp (llist_sl' p ptr l') m);
+    llist_sel_interp p ptr l' m;
+    match reveal l' with
+    | hd::tl -> pts_to_not_null ptr full_perm hd m
 
-let cons_is_not_null #a ptr =
+let cons_is_not_null #a p ptr =
   let h = get () in
-  let l = hide (v_llist ptr h) in
-  extract_info (llist ptr) l (ptr =!= null_llist) (lemma_cons_not_null ptr l)
+  let l = hide (v_llist p ptr h) in
+  extract_info (llist p ptr) l (ptr =!= null_t) (lemma_cons_not_null p ptr l)
 
-let intro_cons_lemma_aux (#a:Type0) (ptr1 ptr2:t a)
+let intro_cons_lemma_aux (#a:Type0) (p : a -> vprop) (ptr1 ptr2:t a)
   (x: cell a) (l:list (cell a)) (m:mem) : Lemma
-  (requires interp (pts_to_sl ptr1 full_perm x `Mem.star` llist_sl' ptr2 l) m /\
-    next x == ptr2)
-  (ensures interp (llist_sl' ptr1 (x::l)) m)
-  = affine_star (pts_to_sl ptr1 full_perm x) (llist_sl' ptr2 l) m;
-    pts_to_not_null ptr1 full_perm x m;
-    emp_unit (pts_to_sl ptr1 full_perm x `Mem.star` llist_sl' ptr2 l);
-    pure_star_interp
-      (pts_to_sl ptr1 full_perm x `Mem.star` llist_sl' ptr2 l)
-      (ptr1 =!= null_llist)
-      m
+  (requires
+    interp (
+      pts_to_sl ptr1 full_perm x `Mem.star`
+      llist_sl' p ptr2 l `Mem.star`
+      hp_of (p (get_data x))) m /\
+    get_next x == ptr2)
+  (ensures (let new_l = x::l in
+    interp (llist_sl' p ptr1 new_l) m))
+  =
+  ()
 
-let intro_cons_lemma (#a:Type0) (ptr1 ptr2:t a)
+let intro_cons_lemma (#a:Type0) (p : a -> vprop) (ptr1 ptr2:t a)
   (x: cell a) (l:list a) (m:mem) : Lemma
-  (requires interp (ptr ptr1 `Mem.star` llist_sl ptr2) m /\
-    next x == ptr2 /\
+  (requires
+    interp (
+      ptr ptr1 `Mem.star`
+      llist_sl p ptr2 `Mem.star`
+      hp_of (p (get_data x))
+    ) m /\
+    get_next x == ptr2 /\
     sel_of (vptr ptr1) m == x /\
-    sel_of (llist ptr2) m == l)
-  (ensures interp (llist_sl ptr1) m /\ llist_sel ptr1 m == data x :: l)
-  = let l' = id_elim_exists (llist_sl' ptr2) m in
-    let aux (m:mem) (x:cell a) (ml mr:mem) : Lemma
-      (requires disjoint ml mr /\ m == join ml mr /\
-        interp (ptr ptr1) ml /\ interp (llist_sl ptr2) mr /\
-        ptr_sel ptr1 m == x /\ interp (llist_sl' ptr2 l') m)
-      (ensures interp (pts_to_sl ptr1 full_perm x `Mem.star` llist_sl' ptr2 l') m)
-      = ptr_sel_interp ptr1 ml;
-        assert (interp (pts_to_sl ptr1 full_perm x) ml);
-        let l2 = id_elim_exists (llist_sl' ptr2) mr in
-        join_commutative ml mr;
-        assert (interp (llist_sl' ptr2 l2) m);
-        llist_sl'_witinv ptr2;
-        assert (interp (llist_sl' ptr2 l') mr);
-        intro_star (pts_to_sl ptr1 full_perm x) (llist_sl' ptr2 l') ml mr
-    in
-    elim_star (ptr ptr1) (llist_sl ptr2) m;
-    Classical.forall_intro_2 (Classical.move_requires_2 (aux m x));
-    assert (interp (pts_to_sl ptr1 full_perm x `Mem.star` llist_sl' ptr2 l') m);
-    intro_cons_lemma_aux ptr1 ptr2 x l' m;
-    intro_h_exists (x::l') (llist_sl' ptr1) m;
-    llist_sel_interp ptr1 (x::l') m
+    sel_of (llist p ptr2) m == l)
+  (ensures interp (llist_sl p ptr1) m /\ llist_sel p ptr1 m == get_data x :: l)
+  =
+  let l' = id_elim_exists (llist_sl' p ptr2) m in
+  //let p1 = pts_to_sl ptr full_perm hd in
+  let p1 = ptr ptr1 in
+  //let p2 = llist_sl' p (get_next hd) tl in
+  let p2 = llist_sl p ptr2 in
+  //let p3 = hp_of (p (get_data hd)) in
+  let p3 = hp_of (p (get_data x)) in
+  let m12, m3 = id_elim_star (p1 `Mem.star` p2) p3 m in
+  let m1, m2 = id_elim_star p1 p2  m12 in
+  // #1
+  ptr_sel_interp ptr1 m1;
+  // #2
+  let l2 = id_elim_exists (llist_sl' p ptr2) m in
+  join_commutative m1 m2;
+  assert (interp (llist_sl' p ptr2 l2) m);
+  llist_sl'_witinv p ptr2;
+  assert (l2 == l');
+  assert (interp (llist_sl' p ptr2 l') m2);
+  // #3
 
-let intro_llist_cons ptr1 ptr2 =
+  intro_star
+    (pts_to_sl ptr1 full_perm x)
+    (llist_sl' p ptr2 l')
+    m1 m2;
+  intro_star
+    (pts_to_sl ptr1 full_perm x `Mem.star`
+    llist_sl' p ptr2 l')
+    (hp_of (p (get_data x)))
+    m12 m3;
+
+  intro_cons_lemma_aux p ptr1 ptr2 x l' m;
+  intro_h_exists (x::l') (llist_sl' p ptr1) m;
+  llist_sel_interp p ptr1 (x::l') m;
+  ()
+
+
+val intro_llist_cons (#a:Type0) (p : a -> vprop)
+  (ptr1 ptr2:t a) (x: a)
+  //(y: t_of (p (get_data x)))
+  : Steel unit
+  (vptr ptr1 `star`
+  llist p ptr2 `star`
+  p x)
+  (fun _ -> llist p ptr1)
+  (requires fun h ->
+    get_next (sel ptr1 h) == ptr2 /\
+    x == get_data (sel ptr1 h)
+    ///\
+    //y == sel (sel_of (p (get_data x))) h
+  )
+  (ensures fun h0 _ h1 ->
+  v_llist p ptr1 h1 == (get_data (sel ptr1 h0)) :: v_llist p ptr2 h0)
+
+let intro_llist_cons p ptr1 ptr2 x =
+  //admit ();
   let h = get () in
-  let x = hide (sel ptr1 h) in
-  let l = hide (v_llist ptr2 h) in
-  reveal_star (vptr ptr1) (llist ptr2);
-  change_slprop (vptr ptr1 `star` llist ptr2) (llist ptr1) (reveal x, reveal l) (data x :: l) (fun m ->  intro_cons_lemma ptr1 ptr2 x l m)
+  let x' = hide (sel ptr1 h) in
+  assert (get_data (reveal x') == x);
+  let l = hide (v_llist p ptr2 h) in
+  //let m = rmem (p (get_data x)) in
+  //let vp = p (get_data x) in
 
-let reveal_non_empty_lemma (#a:Type) (ptr:t a) (l:list (cell a)) (m:mem) : Lemma
-    (requires interp (llist_sl ptr) m /\ llist_sel_cell ptr m == l /\ ptr =!= null_llist)
+  change_slprop_rel
+  (p x)
+  (p (get_data x'))
+  (fun x y -> x == y) (fun _ -> ());
+
+  //let the_p =
+  let m = gget
+    (vptr ptr1 `star`
+    llist p ptr2 `star`
+    p (get_data x')) in
+  //slassert the_p;
+  //let m =
+  //let m = gget vp in
+
+  //let z = gget vp in
+
+  //let sp = sel_of vp in
+  //let hp = rmem vp in
+  //let z = (sel_of vp) (hmem vp) in
+  //let z = fun m -> sel_of vp m in
+
+
+  //let z = hide (sel_of (p (get_data x)) m) in
+  //let z : Ghost.erased (t_of)
+  //reveal_star (vptr ptr1) (llist p ptr2);
+  change_slprop
+    (vptr ptr1 `star`
+    llist p ptr2 `star`
+    p (get_data x'))
+    (llist p ptr1)
+    m
+    //((reveal x, reveal l),
+    //  ())
+      //fun m -> sel_of vp m)
+
+      //fun  -> ())
+      //get_data x)
+      //(reveal h) (p (get_data x)))
+      //sel_of (p (get_data x)))
+      //z)
+      //normal (sel_of (p (get_data x))))
+      //reveal (get_data x))
+    (get_data x' :: l)
+  (fun m -> intro_cons_lemma p ptr1 ptr2 x' l m)
+
+val intro_llist_cons2 (#a:Type0) (p : a -> vprop)
+  (ptr1 ptr2:t a)
+  //(y: t_of (p (get_data x)))
+  : Steel unit
+  (vptr ptr1 `star`
+  llist p ptr2 `star`
+  p (get_data x))
+  (fun _ -> llist p ptr1)
+  (requires fun h ->
+    get_next (sel ptr1 h) == ptr2 /\
+    x == sel ptr1 h
+    ///\
+    //y == sel (sel_of (p (get_data x))) h
+  )
+  (ensures fun h0 _ h1 ->
+  v_llist p ptr1 h1 == (get_data (sel ptr1 h0)) :: v_llist p ptr2 h0)
+
+
+
+
+let reveal_non_empty_lemma (#a:Type) (p : a -> vprop) (ptr:t a) (l:list (cell a)) (m:mem) : Lemma
+    (requires interp (llist_sl p  ptr) m /\ llist_sel_cell p ptr m == l /\ ptr =!= null_t)
     (ensures Cons? l)
-= let l' = id_elim_exists (llist_sl' ptr) m in
-  llist_sel_interp ptr l' m;
-  pure_interp (ptr == null_llist) m
+= let l' = id_elim_exists (llist_sl' p ptr) m in
+  llist_sel_interp p  ptr l' m;
+  pure_interp (ptr == null_t) m
 
 let is_cons (#a:Type) (l:list a) : prop = match l with
   | [] -> False
   | _ -> True
 
 [@@__steel_reduce__]
-let llist_cell' #a r : vprop' =
-  {hp = llist_sl r;
+let llist_cell' #a p r : vprop' =
+  {hp = llist_sl p r;
    t = list (cell a);
-   sel = llist_sel_cell r}
+   sel = llist_sel_cell p r}
 unfold
-let llist_cell (#a:Type0) (r:t a) = VUnit (llist_cell' r)
+let llist_cell (#a:Type0) p (r:t a) = VUnit (llist_cell' p r)
 
 [@@ __steel_reduce__]
-let v_cell (#a:Type0) (#p:vprop) (r:t a)
-  (h:rmem p{FStar.Tactics.with_tactic selector_tactic (can_be_split p (llist_cell r) /\ True)}) : GTot (list (cell a))
-  = h (llist_cell r)
+let v_cell (#a:Type0) (#p2:vprop) (p : a -> vprop) (r:t a)
+  (h:rmem p2{FStar.Tactics.with_tactic selector_tactic (can_be_split p2 (llist_cell p r) /\ True)}) : GTot (list (cell a))
+  = h (llist_cell p r)
 
-val reveal_non_empty_cell (#a:Type0) (ptr:t a)
-  : Steel unit (llist_cell ptr) (fun _ -> llist_cell ptr)
-             (requires fun _ -> ptr =!= null_llist)
-             (ensures fun h0 _ h1 -> v_cell ptr h0 == v_cell ptr h1 /\ Cons? (v_cell ptr h0))
+val reveal_non_empty_cell (#a:Type0) (p : a -> vprop) (ptr:t a)
+  : Steel unit (llist_cell p ptr) (fun _ -> llist_cell p ptr)
+             (requires fun _ -> ptr =!= null_t)
+             (ensures fun h0 _ h1 -> v_cell p ptr h0 == v_cell p ptr h1 /\ Cons? (v_cell p ptr h0))
 
-let reveal_non_empty_cell #a ptr =
+let reveal_non_empty_cell #a p ptr =
   let h = get () in
-  let l = hide (v_cell ptr h) in
-  extract_info (llist_cell ptr) l (is_cons l) (reveal_non_empty_lemma ptr l)
+  let l = hide (v_cell p ptr h) in
+  extract_info (llist_cell p ptr) l (is_cons l) (reveal_non_empty_lemma p ptr l)
 
-let tail_cell_lemma (#a:Type0) (r:t a) (l:list (cell a)) (m:mem) : Lemma
-  (requires Cons? l /\ interp (llist_sl r) m /\ llist_sel_cell r m == l)
+let tail_cell_lemma (#a:Type0) (p : a -> vprop) (r:t a) (l:list (cell a)) (m:mem) : Lemma
+  (requires Cons? l /\ interp (llist_sl p r) m /\ llist_sel_cell p r m == l)
   (ensures (let x = L.hd l in
-    interp (ptr r `Mem.star` llist_sl (next x)) m /\
+    interp (ptr r `Mem.star` llist_sl p (get_next x)) m /\
     sel_of (vptr r) m == x /\
-    sel_of (llist_cell (next x)) m == L.tl l))
-  = llist_sel_interp r l m;
-    assert (interp (llist_sl' r l) m);
+    sel_of (llist_cell p (get_next x)) m == L.tl l))
+  = llist_sel_interp p r l m;
+    assert (interp (llist_sl' p r l) m);
     let x = L.hd l in
     let tl = L.tl l in
-    let sl = pts_to_sl r full_perm x `Mem.star` llist_sl' (next x) tl in
-    pure_star_interp sl (r =!= null_llist) m;
+    let sl = pts_to_sl r full_perm x `Mem.star` llist_sl' p (get_next x) tl in
+    pure_star_interp sl (r =!= null_t) m;
     emp_unit sl;
     assert (interp sl m);
     let aux (m:mem) (ml mr:mem) : Lemma
       (requires disjoint ml mr /\ m == join ml mr /\
-        interp (pts_to_sl r full_perm x) ml /\ interp (llist_sl' (next x) tl) mr)
-      (ensures interp (ptr r `Mem.star` llist_sl (next x)) m /\
+        interp (pts_to_sl r full_perm x) ml /\ interp (llist_sl' p (get_next x) tl) mr)
+      (ensures interp (ptr r `Mem.star` llist_sl p (get_next x)) m /\
         sel_of (vptr r) m == x /\
-        sel_of (llist_cell (next x)) m == tl)
+        sel_of (llist_cell p (get_next x)) m == tl)
       = intro_ptr_interp r (hide x) ml;
-        llist_sel_interp (next x) tl mr;
-        intro_star (ptr r) (llist_sl (next x)) ml mr;
+        llist_sel_interp p (get_next x) tl mr;
+        intro_star (ptr r) (llist_sl p (get_next x)) ml mr;
         ptr_sel_interp r ml;
         pts_to_witinv r full_perm;
         join_commutative ml mr
     in
-    elim_star (pts_to_sl r full_perm x) (llist_sl' (next x) tl) m;
+    elim_star (pts_to_sl r full_perm x) (llist_sl' p (get_next x) tl) m;
     Classical.forall_intro_2 (Classical.move_requires_2 (aux m))
 
 
-val tail_cell (#a:Type0) (ptr:t a)
-  : Steel (t a) (llist_cell ptr)
-                   (fun n -> vptr ptr `star` llist_cell n)
-                   (requires fun _ -> ptr =!= null_llist)
+val tail_cell (#a:Type0) (p : a -> vprop) (ptr:t a)
+  : Steel (t a) (llist_cell p ptr)
+                   (fun n -> vptr ptr `star` llist_cell p n)
+                   (requires fun _ -> ptr =!= null_t)
                    (ensures fun h0 n h1 ->
-                     Cons? (v_cell ptr h0) /\
-                     n == next (sel ptr h1) /\
-                     sel ptr h1 == L.hd (v_cell ptr h0) /\
-                     v_cell n h1 == L.tl (v_cell ptr h0))
+                     Cons? (v_cell p ptr h0) /\
+                     n == get_next (sel ptr h1) /\
+                     sel ptr h1 == L.hd (v_cell p ptr h0) /\
+                     v_cell p n h1 == L.tl (v_cell p ptr h0))
 
-let tail_cell #a ptr =
+let tail_cell #a p ptr =
   let h = get () in
-  let l = hide (v_cell ptr h) in
-  reveal_non_empty_cell ptr;
+  let l = hide (v_cell p ptr h) in
+  reveal_non_empty_cell p ptr;
   let x = hide (L.hd l) in
-  change_slprop (llist_cell ptr) (vptr ptr `star` llist_cell (next x)) l (reveal x, L.tl l)
-    (fun m -> tail_cell_lemma ptr l m);
-  reveal_star (vptr ptr) (llist_cell (next x));
+  change_slprop (llist_cell p ptr) (vptr ptr `star` llist_cell p (get_next x)) l (reveal x, L.tl l)
+    (fun m -> tail_cell_lemma p ptr l m);
+  reveal_star (vptr ptr) (llist_cell p (get_next x));
   let v = read ptr in
-  change_slprop (llist_cell (next x)) (llist_cell (next v)) (L.tl l) (L.tl l) (fun _ -> ());
-  return (next v)
+  change_slprop (llist_cell p (get_next x)) (llist_cell p (get_next v)) (L.tl l) (L.tl l) (fun _ -> ());
+  return (get_next v)
 
-val to_list_cell (#a:Type0) (ptr:t a)
-  : Steel unit (llist ptr) (fun _ -> llist_cell ptr)
-                  (requires fun _ -> True)
-                  (ensures fun h0 _ h1 -> v_llist ptr h0 == datas (v_cell ptr h1))
+val to_list_cell (#a:Type0) (p : a -> vprop) (ptr:t a)
+  : Steel unit (llist p ptr) (fun _ -> llist_cell p ptr)
+  (requires fun _ -> True)
+  (ensures fun h0 _ h1 -> v_llist p ptr h0 == llist_view (v_cell p ptr h1))
 
-let to_list_cell ptr =
-  change_slprop_rel (llist ptr) (llist_cell ptr) (fun x y -> x == datas y) (fun _ -> ())
+let to_list_cell p ptr =
+  change_slprop_rel (llist p ptr) (llist_cell p ptr)
+  (fun x y -> x == llist_view y) (fun _ -> ())
 
-val from_list_cell (#a:Type0) (ptr:t a)
-  : Steel unit (llist_cell ptr) (fun _ -> llist ptr)
-                  (requires fun _ -> True)
-                  (ensures fun h0 _ h1 -> v_llist ptr h1 == datas (v_cell ptr h0))
+val from_list_cell (#a:Type0) (p : a -> vprop) (ptr:t a)
+  : Steel unit (llist_cell p ptr) (fun _ -> llist p ptr)
+  (requires fun _ -> True)
+  (ensures fun h0 _ h1 -> v_llist p ptr h1 == llist_view (v_cell p ptr h0))
 
-let from_list_cell ptr =
-  change_slprop_rel (llist_cell ptr) (llist ptr) (fun x y -> datas x == y) (fun _ -> ())
+let from_list_cell p ptr =
+  change_slprop_rel (llist_cell p  ptr) (llist p ptr)
+  (fun x y -> llist_view x == y) (fun _ -> ())
 
-#push-options "--fuel 2"
-let tail #a ptr =
-  to_list_cell ptr;
-  let n = tail_cell #a ptr in
-  from_list_cell n;
+//#push-options "--fuel 2"
+let tail #a p ptr =
+  to_list_cell p ptr;
+  let n = tail_cell #a p ptr in
+  from_list_cell p n;
   n
-#pop-options
+//#pop-options
 
+
+(*)
 let ind_llist_sl' (#a:Type0) (r:ref (t a)) (p:t a) : slprop u#1 =
   pts_to_sl r full_perm p `Mem.star` llist_sl p
 let ind_llist_sl (#a:Type0) (r:ref (t a)) = Mem.h_exists (ind_llist_sl' r)
@@ -456,4 +582,3 @@ let pack_ind r p =
   let gl = hide (v_llist p h) in
   change_slprop (vptr r `star` llist p) (ind_llist r) (p, reveal gl) gl (fun m -> pack_ind_lemma r p gl m)
 
-#pop-options
