lib_list/Selectors.LList.fsti
@@ -16,79 +16,84 @@ let t (a:Type0) = ref (cell a)
 
 (* Helpers to manipulate cells while keeping its definition abstract *)
 
-val next (#a:Type0) (c:cell a) : t a
-val data (#a:Type0) (c:cell a) : a
+val get_next (#a:Type0) (c:cell a) : t a
+val get_data (#a:Type0) (c:cell a) : a
 val mk_cell (#a:Type0) (n: t a) (d:a)
   : Pure (cell a)
     (requires True)
     (ensures fun c ->
-      next c == n /\
-      data c == d)
+      get_next c == n /\
+      get_data c == d)
 
 /// The null list pointer
-val null_llist (#a:Type) : t a
+val null_t (#a:Type) : t a
 
 /// Lifting the null pointer check to empty lists
-val is_null (#a:Type) (ptr:t a) : (b:bool{b <==> ptr == null_llist})
+val is_null_t (#a:Type) (ptr:t a) : (b:bool{b <==> ptr == null_t})
 
 /// Separation logic predicate stating that reference [r] points to a valid list in memory
-val llist_sl (#a:Type0) (r:t a) : slprop u#1
+val llist_sl (#a:Type0) (p: a -> vprop) (r: t a): slprop u#1
 /// Selector of a list. Returns an F* list of elements of type [a]
-val llist_sel (#a:Type0) (r:t a) : selector (list a) (llist_sl r)
+
+val llist_sel (#a:Type0) (p : a -> vprop) (r:t a) : selector (list a) (llist_sl p r)
 
 /// Combining the two above into a linked list vprop
 [@@__steel_reduce__]
-let llist' #a r : vprop' =
-  {hp = llist_sl r;
+let llist' #a (p : a -> vprop) r : vprop' =
+  {hp = llist_sl p r;
    t = list a;
-   sel = llist_sel r}
+   sel = llist_sel p r}
 unfold
-let llist (#a:Type0) (r:t a) = VUnit (llist' r)
+let llist (#a:Type0) (p : a -> vprop) (r:t a) = VUnit (llist' p r)
 
 /// A wrapper to access a list selector more easily.
 /// Ensuring that the corresponding llist vprop is in the context is done by
 /// calling a variant of the framing tactic, as defined in Steel.Effect.Common
 [@@ __steel_reduce__]
-let v_llist (#a:Type0) (#p:vprop) (r:t a)
-  (h:rmem p{FStar.Tactics.with_tactic selector_tactic (can_be_split p (llist r) /\ True)}) : GTot (list a)
-  = h (llist r)
+let v_llist (#a:Type0) (#p2:vprop) (p : a -> vprop) (r:t a)
+  //(h:rmem p{FStar.Tactics.with_tactic selector_tactic (can_be_split p (llist r) /\ True)}) : GTot (list a)
+  (h:rmem p2{FStar.Tactics.with_tactic selector_tactic (can_be_split p2 (llist p r) /\ True)}) : GTot (list a)
+  = h (llist p r)
 
 (** Stateful lemmas to fold and unfold the llist predicate **)
 
-val intro_llist_nil (a:Type0)
-  : Steel unit emp (fun _ -> llist (null_llist #a))
+val intro_llist_nil (a:Type0) (p : a -> vprop)
+  : Steel unit emp (fun _ -> llist p (null_t #a))
           (requires fun _ -> True)
-          (ensures fun _ _ h1 -> v_llist #a null_llist h1 == [])
+          (ensures fun _ _ h1 -> v_llist #a p null_t h1 == [])
 
-val elim_llist_nil (#a:Type0) (ptr:t a)
-  : Steel unit (llist ptr) (fun _ -> llist ptr)
-          (requires fun _ -> ptr == null_llist)
+val elim_llist_nil (#a:Type0) (p : a -> vprop) (ptr:t a)
+  : Steel unit (llist p ptr) (fun _ -> llist p ptr)
+          (requires fun _ -> ptr == null_t)
           (ensures fun h0 _ h1 ->
-            v_llist ptr h0 == v_llist ptr h1 /\
-            v_llist ptr h1 == [])
+            v_llist p ptr h0 == v_llist p ptr h1 /\
+            v_llist p ptr h1 == [])
 
-val cons_is_not_null (#a:Type0) (ptr:t a)
-  : Steel unit (llist ptr) (fun _ -> llist ptr)
-             (requires fun h -> Cons? (v_llist ptr h))
+val cons_is_not_null (#a:Type0) (p : a -> vprop) (ptr:t a)
+  : Steel unit (llist p ptr) (fun _ -> llist p ptr)
+             (requires fun h -> Cons? (v_llist p ptr h))
              (ensures fun h0 _ h1 ->
-               v_llist ptr h0 == v_llist ptr h1 /\
-               ptr =!= null_llist)
+               v_llist p ptr h0 == v_llist p ptr h1 /\
+               ptr =!= null_t)
 
-val intro_llist_cons (#a:Type0) (ptr1 ptr2:t a)
-  : Steel unit (vptr ptr1 `star` llist ptr2)
-                  (fun _ -> llist ptr1)
-                  (requires fun h -> next (sel ptr1 h) == ptr2)
-                  (ensures fun h0 _ h1 -> v_llist ptr1 h1 == (data (sel ptr1 h0)) :: v_llist ptr2 h0)
+(*)
+val intro_llist_cons (#a:Type0) (p : a -> vprop) (ptr1 ptr2:t a)
+  : Steel unit (vptr ptr1 `star` llist p ptr2)
+                  (fun _ -> llist p ptr1)
+                  (requires fun h -> get_next (sel ptr1 h) == ptr2)
+                  (ensures fun h0 _ h1 -> v_llist p ptr1 h1 == (get_data (sel ptr1 h0)) :: v_llist p ptr2 h0)
+*)
 
-val tail (#a:Type0) (ptr:t a)
-  : Steel (t a) (llist ptr)
-                   (fun n -> vptr ptr `star` llist n)
-                   (requires fun _ -> ptr =!= null_llist)
+val tail (#a:Type0) (p : a -> vprop) (ptr:t a)
+  : Steel (t a) (llist p ptr)
+                   (fun n -> vptr ptr `star` llist p n)
+                   (requires fun _ -> ptr =!= null_t)
                    (ensures fun h0 n h1 ->
-                     Cons? (v_llist ptr h0) /\
-                     sel ptr h1 == mk_cell n (L.hd (v_llist ptr h0)) /\
-                     v_llist n h1 == L.tl (v_llist ptr h0))
+                     Cons? (v_llist p ptr h0) /\
+                     sel ptr h1 == mk_cell n (L.hd (v_llist p ptr h0)) /\
+                     v_llist p n h1 == L.tl (v_llist p ptr h0))
 
+(*)
 (** A variant of lists with an additional indirection pointer to enable in-place operations **)
 
 val ind_llist_sl (#a:Type0) (r:ref (t a)) : slprop u#1
